Scalars.v
@@ -115,7 +115,7 @@ Qed.
 
 Hint Rewrite Scalar_X_Z_triple_1_sqrt_2 Scalar_X_alpha_Z_PI_sqrt_2 Scalar_X_alpha_Z_0_sqrt_2 Scalar_Z_PI_0 Scalar_Z_0_2 Scalar_Z_general : zx_scalar_db.
 
-Lemma Scalar_1_div_sqrt_2_sqrt_identity : ZX_semantics (Stack Scalar_1_div_sqrt_2 Scalar_sqrt_2) = ZX_semantics Empty.
+Lemma Scalar_1_div_sqrt_2_sqrt_identity : ZX_semantics (Stack Scalar_1_div_sqrt_2 Scalar_sqrt_2) = ZX_semantics ⦰.
 Proof.
   simpl.
   autorewrite with zx_scalar_db.
